got the beta rule to work, yay!

theories/OExpr.v
@@ -29,6 +29,7 @@ Defined.
 
 (* Typeclasses Transparent OType_CtxElem. *)
 
+(*
 Definition ctxHead ctx : Type :=
   match ctx with
   | CNil => unit
@@ -46,6 +47,7 @@ Definition ctxTail ctx :=
   | CNil => CNil
   | ctx' :> _ => ctx'
   end.
+*)
 
 
 (***
@@ -66,8 +68,7 @@ Inductive OVar : Ctx -> forall A `{OType A}, Type :=
 .
 
 (* The last-bound variable in a context *)
-Definition var_top {ctx A} `{OType A} : OExpr (ctx :> A) A :=
-  {| ofun_app := snd; ofun_Proper := _ |}.
+Definition var_top {ctx A} `{OType A} : OExpr (ctx :> A) A := snd_ofun.
 
 (* Weaken an OExpr by adding a type to the context *)
 Definition weaken1 {ctx A B} `{OType A} `{OType B}
@@ -84,203 +85,6 @@ Coercion varSemantics : OVar >-> OExpr.
 
 
 (***
- *** Weakening
- ***)
-
-(* Inductive proof that ctx1 can be weakened to ctx2 *)
-Inductive weakensTo ctx1 : Ctx -> Type :=
-| WeakensRefl : weakensTo ctx1 ctx1
-| WeakensCons {ctx2} (w: weakensTo ctx1 ctx2) A `{OType A}  :
-    weakensTo ctx1 (ctx2 :> A)
-.
-
-Arguments WeakensRefl {_}.
-Arguments WeakensCons {_ _} w A {_}.
-
-(* Typeclass version of the above *)
-Class WeakensTo ctx1 ctx2 : Type :=
-  weakensProof : weakensTo ctx1 ctx2.
-
-Instance WeakensTo_refl ctx : WeakensTo ctx ctx := WeakensRefl.
-
-Instance WeakensTo_cons ctx1 ctx2 A `{OType A} (w: WeakensTo ctx1 ctx2) :
-  WeakensTo ctx1 (ctx2 :> A) :=
-  WeakensCons w A.
-
-(* Weaken a context by mapping backwardds from the weaker to the stronger one *)
-Fixpoint weakenContext {ctx1 ctx2} (w: weakensTo ctx1 ctx2) :
-  CtxElem ctx2 -o> CtxElem ctx1 :=
-  match w in weakensTo _ ctx2 return CtxElem ctx2 -o> CtxElem ctx1 with
-  | WeakensRefl => id_ofun
-  | WeakensCons w' _ => compose_ofun fst_ofun (weakenContext w')
-  end.
-
-(* Weakening for OExprs *)
-Definition weakenExpr {ctx1 ctx2} `{w: WeakensTo ctx1 ctx2} {A} `{OType A}
-           (e: OExpr ctx1 A) : OExpr ctx2 A :=
-  compose_ofun (weakenContext w) e.
-
-Instance Proper_weakenExpr {ctx1 ctx2} `{w: WeakensTo ctx1 ctx2} {A} `{OType A} :
-  Proper (oleq ==> oleq) (weakenExpr (w:=w) (A:=A)).
-Proof.
-  intros e1 e2 Re. apply Proper_compose_ofun; [ reflexivity | assumption ].
-Qed.
-
-(* Weakening for variables *)
-Fixpoint weakenVar_h {ctx1 ctx2} (w: weakensTo ctx1 ctx2) :
-  forall {A} `{OType A}, OVar ctx1 A -> OVar ctx2 A :=
-  match w in weakensTo _ ctx2
-        return forall {A} `{OType A}, OVar ctx1 A -> OVar ctx2 A
-  with
-  | WeakensRefl => fun _ _ v => v
-  | WeakensCons w' _ => fun _ _ v => OVar_S (weakenVar_h w' v)
-  end.
-
-Definition weakenVar {ctx1 ctx2} `{w:WeakensTo ctx1 ctx2} {A} `{OType A}
-           (v:OVar ctx1 A) : OVar ctx2 A :=
-  weakenVar_h w v.
-
-(* Weakening is the same whether we do it before or after varSemantics *)
-Lemma weakenVar_weakenExpr {ctx1 ctx2} `{w:WeakensTo ctx1 ctx2} {A} `{OType A}
-      (v:OVar ctx1 A) : weakenExpr (w:=w) v =o= weakenVar v.
-Proof.
-  revert v; induction w; intro v; simpl.
-  { apply id_compose_ofun. }
-  { unfold weaken1. rewrite <- IHw. unfold weakenExpr. simpl.
-    rewrite compose_compose_ofun. reflexivity. }
-Qed.
-
-
-(***
- *** Substitution
- ***)
-
-(* A substitution for a single variable in a ctx *)
-Fixpoint CtxSubst ctx : Type :=
-  match ctx with
-  | CNil => False
-  | ctx' :> A => CtxSubst ctx' + OExpr ctx' A
-  end.
-
-(* The output context of a substitution *)
-Fixpoint CtxSubstCtx {ctx} : CtxSubst ctx -> Ctx :=
-  match ctx return CtxSubst ctx -> Ctx with
-  | CNil => fun empty => match empty with end
-  | ctx' :> A => fun subst_or_expr =>
-                   match subst_or_expr with
-                   | inl subst' => CtxSubstCtx subst' :> A
-                   | inr _ => ctx'
-                   end
-  end.
-
-(* The output type of a substitution *)
-Fixpoint CtxSubstType {ctx} : CtxSubst ctx -> Type :=
-  match ctx return CtxSubst ctx -> Type with
-  | CNil => fun empty => match empty with end
-  | ctx' :> A => fun subst_or_expr =>
-                   match subst_or_expr with
-                   | inl subst' => CtxSubstType subst'
-                   | inr _ => A
-                   end
-  end.
-
-Fixpoint CtxSubstOType {ctx} : forall s, OType (@CtxSubstType ctx s) :=
-  match ctx return forall s, OType (@CtxSubstType ctx s) with
-  | CNil => fun empty => match empty with end
-  | ctx' :> A => fun subst_or_expr =>
-                   match subst_or_expr with
-                   | inl subst' => CtxSubstOType subst'
-                   | inr _ => _
-                   end
-  end.
-
-Instance OType_CtxSubstType ctx s : OType (@CtxSubstType ctx s) :=
-  CtxSubstOType s.
-
-(* Use a substitution like a mapping *)
-Fixpoint substContext {ctx} :
-  forall (s: CtxSubst ctx), CtxElem (CtxSubstCtx s) -o> CtxElem ctx :=
-  match ctx return forall (s: CtxSubst ctx), CtxElem (CtxSubstCtx s) -o>
-                                             CtxElem ctx
-  with
-  | CNil => fun empty => match empty with end
-  | ctx' :> A =>
-    fun s =>
-      match s return CtxElem (@CtxSubstCtx (_ :> _) s) -o> CtxElem (_ :> _) with
-      | inl s' => pair_ofun (compose_ofun fst_ofun (substContext s')) snd_ofun
-      | inr e => pair_ofun id_ofun e
-      end
-  end.
-
-Definition substExpr {ctx A} `{OType A} (e: OExpr ctx A) (s: CtxSubst ctx) :
-  OExpr (CtxSubstCtx s) A :=
-  compose_ofun (substContext s) e.
-
-(* The result of looking up a variable in a substitution; see substVarLookup *)
-Inductive VarLookupRes ctx A `{OType A} (s:CtxSubst ctx) : Type :=
-| mkVarLookupRes ctx' (w: weakensTo ctx' (CtxSubstCtx s))
-                 (v_or_e: OVar ctx' A + OExpr ctx' A) :
-    VarLookupRes ctx A s.
-
-(* Weaken a VarLookupRes *)
-Definition weakenVarLookupRes {ctx A B} `{OType A} `{OType B} {s}
-           (res: VarLookupRes ctx A s) :
-  VarLookupRes (ctx :> B) A (inl s) :=
-  match res with
-  | mkVarLookupRes _ _ _ ctx' w v_or_e =>
-    mkVarLookupRes (_:>_) A (inl s) ctx' (WeakensCons w B) v_or_e
-  end.
-
-(* Look up a variable in a substitution, getting either an OExpr or a
-strengthened variable. We existentially quantify over the returned context so
-that we can do one combined weakening, either of the returned variable or oexpr,
-rather than having N weakening steps *)
-Program Fixpoint substVarLookup {ctx A} `{OType A} (v: OVar ctx A) :
-  forall (s:CtxSubst ctx), VarLookupRes ctx A s :=
-  match v in OVar ctx A return forall s, VarLookupRes ctx A s with
-  | OVar_0 =>
-    fun (s: CtxSubst (_ :> _)) =>
-      match s return VarLookupRes (_:>_) _ s
-      with
-      | inl s' =>
-        mkVarLookupRes (_:>_) _ (inl s') _ WeakensRefl (inl OVar_0)
-      | inr e =>
-        mkVarLookupRes (_:>_) _ (inr e) _ WeakensRefl (inr e)
-      end
-  | OVar_S v' =>
-    fun (s: CtxSubst (_:>_)) =>
-      match s return VarLookupRes (_:>_) _ s with
-      | inl s' =>
-        weakenVarLookupRes (substVarLookup v' s')
-      | inr e =>
-        mkVarLookupRes (_:>_) _ (inr e) _ WeakensRefl (inl v')
-      end
-  end.
-
-(* Substitute into a variable *)
-Definition substVar {ctx A} `{OType A} (v: OVar ctx A) (s:CtxSubst ctx) :
-  OExpr (CtxSubstCtx s) A :=
-  match substVarLookup v s with
-  | mkVarLookupRes _ _ _ ctx' w (inl v') => weakenVar_h w v'
-  | mkVarLookupRes _ _ _ ctx' w (inr e) => weakenExpr (w:=w) e
-  end.
-
-(* Substitution is the same whether we do it before or after varSemantics *)
-Lemma substVar_substExpr {ctx} {A} `{OType A} (v: OVar ctx A)
-      (s: CtxSubst ctx) : substExpr v s =o= substVar v s.
-Proof.
-  revert s; induction v; intro s; unfold substExpr.
-  { destruct s as [ s | e ]; simpl; apply funOExt; intro c; reflexivity. }
-  { destruct s as [ s | e ]; simpl; apply funOExt; intro c; [ | reflexivity ].
-    simpl.
-    assert ((substVar (OVar_S v) (inl s)) = weakenExpr (substVar v s)).
-    - unfold substVar. simpl. destruct (substVarLookup v s); simpl.
-      destruct v_or_e; admit.
-    - rewrite H1. rewrite <- IHv. reflexivity. }
-Admitted.
-
-
-(***
  *** Notation for Application
  ***)
 
@@ -288,6 +92,12 @@ Admitted.
 Definition oexpr_apply {ctx A B} `{OType A} `{OType B}
            (f: OExpr ctx (A -o> B)) (g: OExpr ctx A) : OExpr ctx B :=
   ofun_apply f g.
+
+Instance Proper_oexpr_apply {ctx A B} `{OType A} `{OType B} :
+  Proper (oleq ==> oleq ==> oleq) (@oexpr_apply ctx A B _ _).
+Proof.
+  intros f1 f2 Rf g1 g2 Rg. rewrite Rf. rewrite Rg. reflexivity.
+Qed.
 
 (* Application *)
 Notation "x @o@ y" :=
@@ -305,10 +115,11 @@ Definition oexpr {A} `{OType A} (e: OExpr CNil A) : A := ofun_app e tt.
 Definition oconst {ctx A} `{OType A} (a:A) : OExpr ctx A :=
   const_ofun a.
 
-(* Weaken a variable after coercing it to an expression *)
-(* FIXME: should this specifically be for variables, not exprs? *)
-Definition ovar {ctx A} `{OType A} {ctx'} `{w:WeakensTo ctx ctx'}
-           (e:OExpr ctx A) : OExpr ctx' A := weakenExpr e.
+Instance Proper_oconst {ctx A} `{OType A} :
+  Proper (oleq ==> oleq) (@oconst ctx A _).
+Proof.
+  intros a1 a2 Ra c1 c2 Rc. simpl. assumption.
+Qed.
 
 (* Helper function to build lambdas *)
 (*
@@ -319,17 +130,424 @@ Definition mkLam {ctx A B} `{OType A} `{OType B}
   ofun_curry (body (fun _ _ => weakenVar OVar_0)).
  *)
 
+(*
 Definition mkLam {ctx A B} `{OType A} `{OType B}
            (body : OVar (ctx :> A) A -> OExpr (ctx :> A) B) :
   OExpr ctx (A -o> B) := ofun_curry (body OVar_0).
+ *)
+
+Definition mkLam {ctx A B} `{OType A} `{OType B}
+           (body : OExpr (ctx :> A) A -> OExpr (ctx :> A) B) :
+  OExpr ctx (A -o> B) := ofun_curry (body var_top).
 
 Notation "'ofun' x => e" :=
   (mkLam (fun x => e))
     (right associativity, at level 99).
 
 Notation "'ofun' ( x : A ) => e" :=
-  (mkLam (fun (x : OVar _ A) => e))
+  (mkLam (fun (x : OExpr _ A) => e))
     (right associativity, at level 99, x at level 0).
+
+
+(***
+ *** Weakening
+ ***)
+
+(* Inductive proof that ctx1 can be extended to ctx2 *)
+Inductive extendsTo ctx1 : Ctx -> Type :=
+| ExtendsRefl : extendsTo ctx1 ctx1
+| ExtendsCons {ctx2} (ext: extendsTo ctx1 ctx2) A `{OType A}  :
+    extendsTo ctx1 (ctx2 :> A)
+.
+
+Arguments ExtendsRefl {_}.
+Arguments ExtendsCons {_ _} ext A {_}.
+
+(* Typeclass version of the above *)
+Class ExtendsTo ctx1 ctx2 : Type :=
+  extendsProof : extendsTo ctx1 ctx2.
+
+Instance ExtendsToRefl ctx : ExtendsTo ctx ctx := ExtendsRefl.
+
+Instance ExtendsToCons {ctx1 ctx2} (ext: ExtendsTo ctx1 ctx2) A `{OType A} :
+  ExtendsTo ctx1 (ctx2 :> A) :=
+  ExtendsCons ext A.
+
+(* Weaken a context by mapping backwards from the weaker to the stronger one *)
+Fixpoint weakenContext {ctx1 ctx2} (ext: extendsTo ctx1 ctx2) :
+  CtxElem ctx2 -o> CtxElem ctx1 :=
+  match ext in extendsTo _ ctx2 return CtxElem ctx2 -o> CtxElem ctx1 with
+  | ExtendsRefl => id_ofun
+  | ExtendsCons ext' _ => compose_ofun fst_ofun (weakenContext ext')
+  end.
+
+(* Weakening for OExprs *)
+Definition weakenExpr {ctx1 ctx2} `{ext: ExtendsTo ctx1 ctx2} {A} `{OType A}
+           (e: OExpr ctx1 A) : OExpr ctx2 A :=
+  compose_ofun (weakenContext ext) e.
+
+Instance Proper_weakenExpr {ctx1 ctx2} `{ext: ExtendsTo ctx1 ctx2} {A} `{OType A} :
+  Proper (oleq ==> oleq) (weakenExpr (ext:=ext) (A:=A)).
+Proof.
+  intros e1 e2 Re. apply Proper_compose_ofun; [ reflexivity | assumption ].
+Qed.
+
+Lemma weakenExpr_App {ctx1 ctx2} (ext: ExtendsTo ctx1 ctx2)
+      {A B} `{OType A} `{OType B} (e1: OExpr ctx1 (A -o> B)) (e2: OExpr ctx1 A) :
+  weakenExpr (e1 @o@ e2) =o= weakenExpr e1 @o@ weakenExpr e2.
+  unfold weakenExpr, oexpr_apply. rewrite compose_ofun_apply.
+  reflexivity.
+Qed.
+
+
+(* Weakening for variables *)
+Fixpoint weakenVar_h {ctx1 ctx2} (ext: extendsTo ctx1 ctx2) :
+  forall {A} `{OType A}, OVar ctx1 A -> OVar ctx2 A :=
+  match ext in extendsTo _ ctx2
+        return forall {A} `{OType A}, OVar ctx1 A -> OVar ctx2 A
+  with
+  | ExtendsRefl => fun _ _ v => v
+  | ExtendsCons ext' _ => fun _ _ v => OVar_S (weakenVar_h ext' v)
+  end.
+
+Definition weakenVar {ctx1 ctx2} `{ext:ExtendsTo ctx1 ctx2} {A} `{OType A}
+           (v:OVar ctx1 A) : OVar ctx2 A :=
+  weakenVar_h ext v.
+
+(* Weakening is the same whether we do it before or after varSemantics *)
+Lemma weakenVar_weakenExpr {ctx1 ctx2} `{ext:ExtendsTo ctx1 ctx2} {A} `{OType A}
+      (v:OVar ctx1 A) : weakenExpr (ext:=ext) v =o= weakenVar v.
+Proof.
+  revert v; induction ext; intro v; simpl.
+  { apply id_compose_ofun. }
+  { unfold weaken1. rewrite <- IHext. unfold weakenExpr. simpl.
+    rewrite compose_compose_ofun. reflexivity. }
+Qed.
+
+
+(* Convert a "variable" (an OExpr in a shorter context) into an expression in
+the current context *)
+Definition ovar {ctx A} `{OType A} {ctx'} `{ext:ExtendsTo ctx ctx'}
+           (e:OExpr ctx A) : OExpr ctx' A := weakenExpr e.
+
+
+(***
+ *** Substitution
+ ***)
+
+Inductive CtxSubst : Ctx -> Ctx -> Type :=
+| CtxSubstBase {ctx A} `{OType A} (e: OExpr ctx A) : CtxSubst (ctx :> A) ctx
+| CtxSubstCons {ctx1 ctx2} (s: CtxSubst ctx1 ctx2) A `{OType A} :
+    CtxSubst (ctx1 :> A) (ctx2 :> A)
+.
+
+(* Use a substitution like a mapping *)
+Fixpoint substContext {ctx1 ctx2} (s: CtxSubst ctx1 ctx2)
+  : CtxElem ctx2 -o> CtxElem ctx1 :=
+  match s in CtxSubst ctx1 ctx2
+        return CtxElem ctx2 -o> CtxElem ctx1
+  with
+  | CtxSubstBase e => pair_ofun id_ofun e
+  | CtxSubstCons s' _ =>
+    pair_ofun (compose_ofun fst_ofun (substContext s')) snd_ofun
+  end.
+
+Definition substExpr {ctx1 ctx2 A} `{OType A} (e: OExpr ctx1 A)
+           (s: CtxSubst ctx1 ctx2) : OExpr ctx2 A :=
+  compose_ofun (substContext s) e.
+
+
+(***
+ *** Typeclasses for Weakening
+ ***)
+
+Inductive PreExtendsTo : Ctx -> Ctx -> Type :=
+| PreExtendsToBase {ctx1 ctx2} (ext: extendsTo ctx1 ctx2) :
+    PreExtendsTo ctx1 ctx2
+| PreExtendsToCons {ctx1 ctx2} (pext: PreExtendsTo ctx1 ctx2) A `{OType A} :
+    PreExtendsTo (ctx1 :> A) (ctx2 :> A)
+.
+
+Fixpoint weakenPreContext {ctx1 ctx2} (pext: PreExtendsTo ctx1 ctx2) :
+  CtxElem ctx2 -o> CtxElem ctx1 :=
+  match pext in PreExtendsTo ctx1 ctx2 return CtxElem ctx2 -o> CtxElem ctx1 with
+  | PreExtendsToBase ext => weakenContext ext
+  | PreExtendsToCons pext' _ =>
+    pair_ofun (compose_ofun fst_ofun (weakenPreContext pext')) snd_ofun
+  end.
+
+Class WeakensTo {ctx ctx_e A} `{OType A} (e: OExpr ctx_e A)
+      (pext: PreExtendsTo ctx_e ctx) (res: OExpr ctx A) :=
+  weakensTo :
+    compose_ofun (weakenPreContext pext) e =o= res.
+
+Instance WeakensTo_Const {ctx ctx_e A} `{OType A}
+         (a:A) (pext: PreExtendsTo ctx_e ctx) :
+  WeakensTo (oconst a) pext (oconst a).
+Proof.
+  apply funOExt; intro celem. reflexivity.
+Qed.
+
+Instance WeakensTo_Refl {ctx A} `{OType A} (e: OExpr ctx A) :
+  WeakensTo e (PreExtendsToBase (ExtendsToRefl ctx)) e.
+Proof.
+  apply id_compose_ofun.
+Qed.
+
+Instance WeakensTo_Trivial {ctx_e ctx A} `{OType A} (e: OExpr ctx_e A)
+         (ext: ExtendsTo ctx_e ctx) :
+  WeakensTo e (PreExtendsToBase ext) (ovar e) | 10.
+Proof.
+  apply id_compose_ofun.
+Qed.
+
+Instance WeakensTo_App {ctx_e ctx A B} `{OType A} `{OType B}
+         (e1: OExpr ctx_e (A -o> B)) e2
+         (pext: PreExtendsTo ctx_e ctx) res1 res2 :
+  WeakensTo e1 pext res1 -> WeakensTo e2 pext res2 ->
+  WeakensTo (e1 @o@ e2) pext (res1 @o@ res2).
+Proof.
+  unfold WeakensTo. intros. rewrite <- H1. rewrite <- H2.
+  unfold oexpr_apply. rewrite compose_ofun_apply.
+  reflexivity.
+Qed.
+
+Instance WeakensTo_Lam {ctx_e ctx A B} `{OType A} `{OType B}
+         (body: OExpr (ctx_e :> A) A -> OExpr (ctx_e :> A) B)
+         (pext: PreExtendsTo ctx_e ctx) body_res :
+  (forall v v_res,
+      WeakensTo v (PreExtendsToCons pext A) v_res ->
+      WeakensTo (body v) (PreExtendsToCons pext A) (body_res v_res)) ->
+  WeakensTo (mkLam body) pext (mkLam body_res).
+Proof.
+  unfold WeakensTo, mkLam.
+  intro pf. rewrite <- (pf var_top var_top).
+  { rewrite compose_ofun_curry. reflexivity. }
+  { simpl. apply compose_pair_snd. }
+Qed.
+
+
+Class WeakensToVar {ctx_e ctx_e_res ctx ctx_res A} `{OType A}
+      (e: OExpr ctx_e A) (ext_v: ExtendsTo ctx_e ctx)
+      (pext: PreExtendsTo ctx ctx_res)
+      (res: OExpr ctx_e_res A) (ext_res: ExtendsTo ctx_e_res ctx_res) :=
+  weakensToVar :
+    compose_ofun (weakenPreContext pext) (ovar e) =o= (ovar res).
+
+Instance WeakensToVar_Refl {ctx_e ctx A} `{OType A}
+         (e: OExpr ctx_e A) (pext: PreExtendsTo ctx_e ctx) res :
+  WeakensTo e pext res ->
+  WeakensToVar e (ExtendsToRefl _) pext res (ExtendsToRefl _).
+Proof.
+  intro pf; apply pf.
+Qed.
+
+Instance WeakensToVar_Const {ctx_e ctx A} `{OType A}
+         (e: OExpr ctx_e A) (ext_v: ExtendsTo ctx_e ctx) :
+  WeakensToVar e ext_v (PreExtendsToBase (ExtendsToRefl _)) e ext_v.
+Proof.
+  apply id_compose_ofun.
+Qed.
+
+Instance WeakensToVar_Cons1 {ctx_e ctx ctx_res ctx_e_res A B} `{OType A} `{OType B}
+         (e: OExpr ctx_e A) (ext_v: ExtendsTo ctx_e ctx)
+         (pext: PreExtendsTo ctx ctx_res)
+         (res: OExpr ctx_e_res A) (ext_res : ExtendsTo ctx_e_res ctx_res) :
+  WeakensToVar e ext_v pext res ext_res ->
+  WeakensToVar e (ExtendsToCons ext_v B)
+               (PreExtendsToCons pext B) res (ExtendsToCons ext_res B).
+Proof.
+  unfold WeakensToVar, ovar, ovar, weakenExpr. simpl.
+  intro pf. repeat rewrite <- compose_compose_ofun. rewrite <- pf.
+  apply funOExt; intro celem. reflexivity.
+Qed.
+
+Instance WeakensToVar_Cons2 {ctx_e ctx ctx_res ctx_e_res A B} `{OType A} `{OType B}
+         (e: OExpr ctx_e A) (ext_v: ExtendsTo ctx_e ctx)
+         (ext: ExtendsTo ctx ctx_res)
+         (res: OExpr ctx_e_res A) (ext_res : ExtendsTo ctx_e_res ctx_res) :
+  WeakensToVar e ext_v (PreExtendsToBase ext) res ext_res ->
+  WeakensToVar e ext_v (PreExtendsToBase (ExtendsToCons ext B))
+               res (ExtendsToCons ext_res B).
+Proof.
+  unfold WeakensToVar, ovar, ovar, weakenExpr. simpl.
+  intro pf. repeat rewrite <- compose_compose_ofun. rewrite <- pf.
+  apply funOExt; intro celem. reflexivity.
+Qed.
+
+
+Instance WeakensTo_Var {ctx_e ctx ctx_e_res ctx_res A} `{OType A}
+         (e: OExpr ctx_e A) (ext_v: ExtendsTo ctx_e ctx)
+         (pext: PreExtendsTo ctx ctx_res)
+         (res: OExpr ctx_e_res A) (ext_res: ExtendsTo ctx_e_res ctx_res) :
+  WeakensToVar e ext_v pext res ext_res ->
+  WeakensTo (ovar e) pext (ovar res).
+Proof.
+  intro pf; apply pf.
+Qed.
+
+
+(***
+ *** Typeclasses for Substitution
+ ***)
+
+Class SubstsTo {ctx ctx_res A} `{OType A} (e: OExpr ctx A)
+      (s: CtxSubst ctx ctx_res) res :=
+  substsTo : substExpr e s =o= res.
+
+Instance SubstsTo_Const {ctx ctx_res A} `{OType A} (a:A)
+         (s: CtxSubst ctx ctx_res) :
+  SubstsTo (oconst a) s (oconst a).
+Proof.
+  apply funOExt; intro celem. reflexivity.
+Qed.
+
+Instance SubstsTo_App {ctx ctx_res A B} `{OType A} `{OType B}
+         (e1: OExpr ctx (A -o> B)) (e2: OExpr ctx A)
+         (s: CtxSubst ctx ctx_res) res1 res2 :
+  SubstsTo e1 s res1 -> SubstsTo e2 s res2 ->
+  SubstsTo (e1 @o@ e2) s (res1 @o@ res2).
+Proof.
+  unfold SubstsTo. unfold substExpr. intros. rewrite <- H1. rewrite <- H2.
+  unfold oexpr_apply. rewrite compose_ofun_apply.
+  reflexivity.
+Qed.
+
+Instance SubstsTo_Lam {ctx ctx_res A B} `{OType A} `{OType B}
+         (body: OExpr (ctx :> A) A -> OExpr (ctx :> A) B)
+         (s: CtxSubst ctx ctx_res)
+         (body_res: OExpr (ctx_res :> A) A -> OExpr (ctx_res :> A) B) :
+  (forall v v_res,
+      SubstsTo v (CtxSubstCons s A) v_res ->
+      SubstsTo (body v) (CtxSubstCons s A) (body_res v_res)) ->
+  SubstsTo (mkLam body) s (mkLam body_res).
+Proof.
+  unfold SubstsTo, substExpr, mkLam. intro pf. rewrite <- (pf var_top var_top).
+  { rewrite compose_ofun_curry. reflexivity. }
+  { simpl. apply compose_pair_snd. }
+Qed.
+
+Class SubstsToVar {ctx ctx_e ctx_res ctx_e_res A} `{OType A}
+      (e: OExpr ctx_e A) (ext: ExtendsTo ctx_e ctx)
+      (s: CtxSubst ctx ctx_res) (res: OExpr ctx_e_res A)
+      (ext_res: ExtendsTo ctx_e_res ctx_res) :=
+  substsToVar : substExpr (ovar (ext:=ext) e) s =o= ovar (ext:=ext_res) res.
+
+Instance SubstsToVar_Refl {ctx ctx_res A} `{OType A}
+         (e: OExpr ctx A) (s: CtxSubst ctx ctx_res) res :
+  SubstsTo e s res -> SubstsToVar e (ExtendsToRefl ctx) s res (ExtendsToRefl _).
+Proof.
+  unfold SubstsTo, SubstsToVar, ovar, ExtendsToRefl, substExpr, weakenExpr.
+  simpl. repeat rewrite id_compose_ofun. intro; assumption.
+Qed.
+
+Instance SubstsToVar_VarSubst {ctx A} `{OType A} (e_subst: OExpr ctx A) :
+  SubstsToVar var_top (ExtendsToRefl _) (CtxSubstBase e_subst)
+              e_subst (ExtendsToRefl _).
+Proof.
+  unfold SubstsTo, SubstsToVar, ovar, var_top.
+  unfold substExpr, weakenExpr, ExtendsToRefl.
+  simpl. repeat rewrite id_compose_ofun. rewrite compose_pair_snd.
+  reflexivity.
+Qed.
+
+Instance SubstsToVar_Const {ctx ctx_e A B} `{OType A} `{OType B}
+         (e: OExpr ctx_e A) (ext: ExtendsTo ctx_e ctx)
+         (e_subst: OExpr ctx B) :
+  SubstsToVar e (ExtendsToCons ext B) (CtxSubstBase e_subst) e ext.
+Proof.
+  unfold SubstsTo, SubstsToVar, ovar, weakenExpr, substExpr. simpl.
+  apply funOExt; intro celem. reflexivity.
+Qed.
+
+Instance SubstsToVar_Cons {ctx_e ctx_e_res ctx ctx_res A B} `{OType A} `{OType B}
+         (e: OExpr ctx_e A) (ext: ExtendsTo ctx_e ctx)
+         (s: CtxSubst ctx ctx_res) (res: OExpr ctx_e_res A) ext_res :
+  SubstsToVar e ext s res ext_res ->
+  SubstsToVar e (ExtendsToCons ext B) (CtxSubstCons s B)
+              res (ExtendsToCons ext_res B).
+Proof.
+  unfold SubstsTo, SubstsToVar, ovar, ovar, weakenExpr, substExpr. simpl.
+  intro pf. repeat rewrite <- compose_compose_ofun. rewrite <- pf.
+  apply funOExt; intro celem. reflexivity.
+Qed.
+
+Instance SubstsTo_Var {ctx ctx_res ctx_e ctx_e_res A} `{OType A}
+         (e: OExpr ctx_e A) (ext: ExtendsTo ctx_e ctx)
+         (s: CtxSubst ctx ctx_res)
+         (res: OExpr ctx_e_res A) (ext_res: ExtendsTo ctx_e_res ctx_res)
+         (res_w: OExpr ctx_res A) :
+  SubstsToVar e ext s res ext_res ->
+  WeakensTo res (PreExtendsToBase ext_res) res_w ->
+  SubstsTo (ovar (ext:=ext) e) s res_w.
+Proof.
+  unfold SubstsTo, SubstsToVar, WeakensTo. intros.
+  etransitivity; eassumption.
+Qed.
+
+
+(***
+ *** Beta and Eta Rules for OFuns
+ ***)
+
+Lemma ofunEta {ctx A B} `{OType A} `{OType B} (e: OExpr ctx (A -o> B)) :
+  (ofun x => ovar e @o@ ovar x) =o= e.
+Proof.
+  apply funOExt; intro celem. apply funOExt; intro a. reflexivity.
+Qed.
+
+Lemma ofunExt {ctx A B} `{OType A} `{OType B} (e1 e2: OExpr ctx (A -o> B))
+      (pf: forall arg, e1 @o@ arg =o= e2 @o@ arg) :
+  e1 =o= e2.
+Proof.
+  apply funOExt; intro celem. unfold oexpr_apply in pf.
+  apply funOExt; intro a. revert celem.
+  rewrite <- (funOExt _ _ (e1 @o@ oconst a) (e2 @o@ oconst a)).
+  apply pf.
+Qed.
+
+Lemma ofunExt_leq {ctx A B} `{OType A} `{OType B} (e1 e2 : OExpr ctx (A -o> B))
+      (pf: forall arg, e1 @o@ arg =o= e2 @o@ arg) :
+  e1 <o= e2.
+Proof.
+  intros c1 c2 Rc a1 a2 Ra. rewrite Rc; rewrite Ra.
+  destruct (pf (oconst a2)). apply H1. reflexivity.
+Qed.
+
+Lemma ofunEta' {ctx A B} `{OType A} `{OType B} (e: OExpr ctx (A -o> B)) :
+  (ofun x => ovar e @o@ x) =o= e.
+Proof.
+  apply funOExt; intro celem. apply funOExt; intro a. reflexivity.
+Qed.
+
+Lemma ofunBeta {ctx A B} `{OType A} `{OType B}
+      (body: OExpr (ctx :> A) A -> OExpr (ctx :> A) B) (arg: OExpr ctx A) res
+      {st:
+         forall v, SubstsTo v (CtxSubstBase arg) arg ->
+                   SubstsTo (body v) (CtxSubstBase arg) res} :
+  (mkLam body) @o@ arg =o= res.
+Proof.
+  unfold SubstsTo in st. rewrite <- (st var_top).
+  { unfold substExpr, mkLam, oexpr_apply. simpl.
+    rewrite ofun_apply_ofun_curry. reflexivity. }
+  { apply compose_pair_snd. }
+Qed.
+
+Ltac obeta := rewrite ofunBeta; [ | typeclasses eauto ].
+
+
+(***
+ *** Tests for the obeta Tactic
+ ***)
+Lemma beta_test {ctx A} `{OType A} (e: OExpr ctx A) :
+  (ofun x => ovar x) @o@ e =o= e.
+  obeta. reflexivity.
+Qed.
+
+Lemma beta_test2 {ctx A B} `{OType A} `{OType B} (e: OExpr ctx (A -o> B)) :
+  (ofun f => (ofun x => ovar f @o@ ovar x)) @o@ e =o= e.
+  obeta. apply ofunExt; intro. obeta. reflexivity.
+Qed.
 
 
 (***
